Add functions sdiv and srem in bitvector theories.
Suitable for SMT solvers with BV support, but not for others: need to add definitional axioms and realize them in Coq and Isabelle

lib/coq/bv/BV_Gen.v
@@ -17,6 +17,7 @@ Require bool.Bool.
 Require int.Int.
 Require int.Abs.
 Require int.EuclideanDivision.
+Require int.ComputerDivision.
 Require bv.Pow2int.
 
 Local Parameter last_bit : nat.
@@ -1610,6 +1611,29 @@ Lemma to_uint_urem :
   apply Mod_bound; trivial.
   rewrite Z.abs_eq; apply to_uint_bounds.
 Qed.
+
+(* abstract sdiv and srem while we have no realization yet *)
+Definition sdiv_abstract : t -> t -> t.
+  admit.
+Admitted.
+
+Definition srem_abstract : t -> t -> t.
+  admit.
+Admitted.
+
+
+
+(* Why3 goal *)
+Definition sdiv : t -> t -> t.
+Proof.
+  exact sdiv_abstract.
+Defined.
+
+(* Why3 goal *)
+Definition srem : t -> t -> t.
+Proof.
+  exact srem_abstract.
+Defined.
 
 (* Why3 goal *)
 Definition lsr_bv : t -> t -> t.
